\begin{problem}
    Let $X_1,\ldots,X_n\sim F$ and let $ F_n(x)$ be the empirical distribution function, for a fixed $x$,  find limiting distribution of $\sqrt{F_n(x)}$.
\end{problem}

\begin{solution}
We have $F_n=\frac{1}{n} \sum_{i=1}^n I(X_i \le x)$, and $F_n (x) \sim \frac{1}{n} Binomial(n, F(x))$.
By CLT, we get $\frac{n F_n(x)- nF(x)}{\sqrt{n}\sqrt{F(x)(1-F(x))}} = \sqrt{n} \frac{F_n(x)- F(x)}{\sqrt(F(x)(1-F(x)))} \leadsto N(0,1)$.
Thus, $\sqrt{n} ( F_n(x)- F(x) ) \leadsto N(0, F(x)(1-F(x)))$. 

According to \emph{Delta Method}, we have $\sqrt{n} (\sqrt{F_n (x)} -\sqrt{F (x)}) \leadsto \frac{\partial \sqrt{F(x)}}{\partial F(x)} N(0, F(x)(1-F(x)))$. 
Finally, we get $\sqrt{F_n} \leadsto N(\sqrt{F(x)}, \frac{1-F(x)}{4n})$.

% Let $T(F)=\sqrt{F}$, we know that $T$ is Hadamard differentiable with respect to $G=\delta_x$. 
% Then
% \begin{equation*}
%     \frac{\sqrt{n} (T (F_n) - T(F))}{\hat{\tau}} \leadsto N(0, 1)
% \end{equation*}
% where $\hat{\tau}^2=\frac{1}{n}\sum_{i=1}^n \hat{L}^2(X_i)$ and
% \begin{equation*}
%     \frac{d}{dt}T(F_t) \Big|_{t=0} 
%     = \frac{d}{dt} \sqrt{F_t} 
%     = \frac{d}{dt} \sqrt{(1-t)F+t\delta_x}
%     =  - \sqrt{F}.
% \end{equation*}

% So, $\hat{\tau} = \sqrt{\frac{1}{n}\sum_{i=1}^n F_n(X_i)} $.

% Thus, $ T (F_n)  \leadsto N(\sqrt{F}, \frac{1}{n^2}\sum_{i=1}^n F_n(X_i))$

\end{solution}





\begin{problem}
    Let $x$, $y$ be two distinct real numbers, find $Cov(F_n(x),F_n(y))$, where $ F_n $ be the empirical distribution function. 
\end{problem}
\begin{solution}
    Assume that $x<y$. 
    We have $F_n (x)=\frac{1}{n} \sum_{i=1}^n I(X_i \le x)$, and $F_n (x)\sim \frac{1}{n} Binomial(n, F(x))$.
    This gives
    \begin{equation*}
        \begin{split}
            Cov(F_n(x),F_n(y)) & = E[F_n (x)-E(F_n (x))][F_n (y)-E(F_n (y))] \\
            % & = E[F_n (x)-F(x)][F_n (y)-F(y)] \\
            & = E[F_n (x) F_n (y)] - E[F_n(x)]E[F_n(y)] \\
            % & = E\left[ \sum_{i=1}^n I(X_i\le x) \sum_{i=1}^n I(X_i\le y) \right] - F(x)F(y) \\
        \end{split}
    \end{equation*} 
    where 
    \begin{equation*}
        \begin{split}
            n^2 E[F_n (x) F_n (y)] & = E\left[ \sum_{i=1}^n I(X_i\le x) \sum_{j=1}^n I(X_j\le y) \right] \\
            & = E\left[  \sum_{i=1}^n \sum_{j=1}^n  I(X_i\le x) I(X_j\le y) \right] \\
            & = \sum_{i=1}^n \sum_{j=1}^n E\left[ I(X_i\le x) I(X_j\le y) \right] \\
            & = \sum_{i=1}^n E\left[ I(X_i\le x)I(X_i\le y) \right] + \sum_{i,j=1; i\neq j}^n  E\left[ I(X_i\le x)\right]  E\left[ I(X_j\le y)\right] \\
            & = n F(x) +  n(n-1)F(x)F(y) 
        \end{split} 
    \end{equation*}
    and 
    $E[F_n(x)]E[F_n(y)] = F(x)F(y)$.

    Thus, $Cov(F_n(x),F_n(y)) = \frac{F(x) +  (n-1)F(x)F(y)}{n} - F(x)F(y) =\frac{F(x) - F(x)F(y)}{n}  $
\end{solution}




\begin{problem}
    Let $ X_{(1)}\le\cdots\le X_{(n)}$ be order statistics from continuous popolation  $F$, prove that for any $0<\beta<1$
    \begin{equation*}
        \mathbf{P}(F(X_{(n)})-F(X_{(1)})>\beta)=1-n\beta^{n-1}+(n-1)\beta^n.
    \end{equation*}
\end{problem}
\begin{solution}
    % We have  $\mathbf{P} \left(F(X_{(n)}) \le x, F(X_{(1)}) \le y \right) =x^n \left(1-(1-y)^n \right)$ which leads to the joint probability density of $F(X_{(n)})$ and $F(X_{(1)})$, 
    % $f_{F(X_{(n)}), F(X_{(1)})} (x,y) = \frac{\partial}{\partial x \partial y} x^n \left(1-(1-y)^n \right) = n^2 x^{n-1} (1-y)^{n-1}$. 
    
    % Thus, $\mathbf{P}( F(X_{(n)})-F(X_{(1)})>\beta ) 
    % = \int_{x-y>\beta} f_{F(X_{(n)}), F(X_{(1)})} (x,y) dxdy 
    % = \int_0^{1-\beta} \int_{y+\beta}^1 n^2 x^{n-1} (1-y)^{n-1} dy dx 
    % = \int_0^{1-\beta} (1-(y-\beta)^n) (1-y)^{n-1} dy 
    % = 1-\beta^n - \int_0^{1-\beta} (y+\beta)^n (1-y)^{n-1} dy 
    % = $
    
    % $F(X_{(n)} $



    We have $ \mathbf{P} (F(X_{(n)})-F(X_{(1)})>\beta) = 1 -  \mathbf{P} (F(X_{(n)})-F(X_{(1)}) \le \beta) $, $F(X_1), \dots, F(X_n)$ have \emph{i.i.d.} standard uniform distribution, $F(X_{(1)}), \dots, F(X_{(n)})$ are ordered statistics, $ F(X_{(n)} - F(X_{(1)})) \sim Beta(n-1, 2)$ and 
    \begin{equation*}
        \begin{split}
            \mathbf{P} (F(X_{(n)})-F(X_{(1)}) \le \beta) & = \int_0^1 n(n-1) x^{n-2} (1-x) dx \\
            % & = \prod_{i\neq j}  \mathbf{P} (F(X_i) - F(X_j) \le \beta) \\
            % & = \prod_{i\neq j} \mathbf{P}  \iint\limits_{F(X_i) - F(X_j) \le \beta} dF(X_i) dF(X_j) \\
            % & =  \left( \frac{1}{2} + \beta - \frac{\beta^2}{2} \right)^{n^2-n} \\
            & = n\beta^{n-1} - (n-1)\beta^n.
        \end{split}
    \end{equation*}

    Thus $ \mathbf{P}(F(X_{(n)})-F(X_{(1)})>\beta)=1-n\beta^{n-1}+(n-1)\beta^n.$
\end{solution}




\begin{problem}
    Let $ X_1,\ldots,X_n $ be simple samples from $U(0,1)$, prove that sample median $\hat\xi_{n,1/2}$ has asymptotic distribution $N(\frac12,\frac{1}{4n})$.
\end{problem}
\begin{solution}
    Let $F$ be the distribution function of $U(0,1)$. 

    $\forall p\in (0,1)$, let $t>0, p_{nt} = F(\xi_{p} + \frac{t\sigma_F}{\sqrt{n}}), c_{nt} = \sqrt{p_{nt}-p} / \sqrt{p_{nt}(1-p_{nt})}$ and $Z_{nt} = [B_n(p_{nt})-np_{nt}]/\sqrt{np_{nt}(1-p_{nt})}$, where $B_n(q)$ denotes a random variable having the binomial distribution $Bi(q,n)$. Then
    \begin{equation*}
        \begin{split}
            \mathbf{P} (\hat{\xi}_{n,p} \le \xi_p + \frac{t\sigma_F}{\sqrt{n}}) & = \mathbf{P} (p \le F_n(\xi_p + \frac{t\sigma_F}{\sqrt{n}})) \\
            & = \mathbf{P} (Z_{nt} \ge -c_{nt}) \\
        \end{split}
    \end{equation*}
    Then $p_{nt}\to p$ and $c_{nt}\to t$. Hence, we get
    \begin{equation*}
        \mathbf{P}(Z_{nt}\le -c_{nt}) -\Phi(-c_{nt}) \to 0
    \end{equation*}
    by CLT and Polya Throrem. Thus 
    \begin{equation*}
        \sqrt{n}(\hat{\xi}_{n,p} - \xi_p) \leadsto N(0,\sigma_F^2).
    \end{equation*}

    We have $F(1/2)=1/2$ and $F'$  exist and is positive at $1/2$. Thus, the result follows from letting $p=1/2$, which gives $\xi_p= 1/2, \sigma_F=1/4$.
\end{solution}
