\begin{problem}[HW 10.2]
Suppose $X_1,\ldots.X_n$ i.i.d obey the unary density $f(x)$. The random variable $U$ obeys a uniform distribution over $\{1,2,...,n\}$, let $Y=X_U+hZ$, where $Z$ has the density $p(x)$ And independent of $X_1,\ldots.X_n$ and $U$.

(1) Prove that under the given conditions of $X_1, \dots,X_n$, $Y$ has a density $\hat{f}(\cdot)$, which is a kernel estimate based on the samples $X_1, \dots,X_n$ and the kernel function $p(\cdot)$ and the bandwidth $h$.

(2) Find the variance of $Y$ given the conditions of $X_1, \dots,X_n$. 
How does it compare with the variance of the samples based on $X_1, \dots,X_n$?

\end{problem}

\begin{solution}
    (1) Firstly, let's focuse on $Y$'s density function $\hat{f}(\cdot)$.

    \begin{equation*}
        \begin{split}
            P(Y < x) & = P(X_U + hZ < y) \\
            & = E\left[ P(X_U + hZ < x | U = i) \right] \\
            & = E \left[ P(Z < \frac{x-X_i}{h}) \right] \\
            & = \frac{1}{n} \sum_{i=1}^n \int_0^{\frac{x-X_i}{h}} p(t) dt \\
        \end{split}
    \end{equation*}
    This leads to 
    \begin{equation*}
        \hat{f}(\cdot) = \frac{1}{n} \sum_{i=1}^n \frac{1}{h} p\left( \frac{x-X_i}{h} \right) 
    \end{equation*}

    Actually, this is the KDE on the samples $X_1, \dots,X_n$ and the kernel function $p(\cdot)$ and the bandwidth $h$.
    
    (2) 
    If we assume $p(\cdot)$ astisfy $\int t p(t) dt = 0$. Then the variance of $Y$ is
    \begin{equation*}
        \begin{split}
            Var(Y) & = \int x^2 \hat{f}(x) dx - \left( \int x\hat{f}(x) dx \right)^2 \\
            & = \int x^2  \frac{1}{n} \sum_{i=1}^n \frac{1}{h} p\left( \frac{x-X_i}{h} \right) dx - \left( \int x  \frac{1}{n} \sum_{i=1}^n \frac{1}{h} p\left( \frac{x-X_i}{h} \right)  dx \right)^2 \\
            & = \frac{1}{nh} \sum_{i=1}^n \int x^2 p\left( \frac{x-X_i}{h} \right) dx - \frac{1}{n^2h^2} \left( \sum_{i=1}^n \int x  p\left( \frac{x-X_i}{h} \right)  dx \right)^2 \\
            & = \frac{1}{nh} \sum_{i=1}^n \int h (ht+X_i)^2 p(t) dt - \frac{1}{n^2h^2} \left( \sum_{i=1}^n \int h(ht+X_i)  p(t)  dt \right)^2 \\
            & = \frac{1}{n} \sum_{i=1}^n \left[ h^2 EZ^2 + 2hX_iEZ + X_i^2 \right] - \frac{1}{n^2}  \left( \sum_{i=1}^n hEZ + X_i \right)^2 \\
            & = h^2 EZ^2 + 2h\bar{X}EZ + \overline{X^2} - \left( \bar{X}^2  + h^2 (EZ)^2 + 2hEZ\bar{X} \right) \\
            & =  \overline{X^2} - \bar{X}^2 + h^2 EZ^2   \\
        \end{split}
    \end{equation*}

    While the sample variance of $X$ is
    \begin{equation*}
        Var_S(X) = \frac{1}{n} \sum_{i=1}^n \left( X_i - \bar{X} \right)^2 = \overline{X^2} - \bar{X}^2
    \end{equation*}

    $Var(Y)$ is a little biger than $Var_S(X)$ about $h^2 EZ^2 \to 0$ if $h\to0$.
\end{solution}